start implementing models for the LoopMonad

state_monad.v
@@ -2,7 +2,7 @@ Require Import ZArith ssreflect ssrmatching ssrfun ssrbool.
 From mathcomp Require Import eqtype ssrnat seq choice fintype tuple.
 From mathcomp Require Import boolp.
 From infotheo Require Import ssrZ.
-Require Import monad.
+From monae Require Import monad.
 
 Set Implicit Arguments.
 Unset Strict Implicit.
@@ -70,6 +70,107 @@ Example test_nonce0 (M : stateMonad nat) : M nat :=
   Get >>= (fun s => Put s.+1 >> Ret s).
 (*Reset test_nonce0.
 Fail Check test_nonce0.*)
+
+(* Module MonadLoop. *)
+(* Record mixin_of (M : monad -> monad) (mo : monad) : Type := Mixin { *)
+(*    lift : forall A, mo A -> M mo A ; *)
+(*    run : forall A, M mo A -> mo A ; *)
+(*    foreach : nat -> nat -> (nat -> M mo unit) -> mo unit ; *)
+(*   _ : forall m n body, foreach m (m + n.+1) body = Ret tt ; *)
+(*   _ : forall m body, foreach m m body = run (body m); *)
+(*   _ : forall m n body, foreach (m.+1 + n) m body = *)
+(*      run (body (m.+1 + n)) >> foreach (m + n) m body :> mo unit *)
+(* }. *)
+
+(* Record class_of (M : monad -> monad) (mo : monad) := Class { *)
+(*   base : Monad.class_of (M mo) ; mixin : mixin_of (Monad.Pack base) mo }. *)
+(* Structure t : Type := Pack { m : Type -> Type ; class : class_of m }. *)
+(* Definition baseType (M : t) := Monad.Pack (base (class M)). *)
+(* Module Exports. *)
+(* Definition Foreach (M : t) : nat -> nat -> (nat -> m M unit) -> m M unit := *)
+(*   let: Pack _ (Class _ (Mixin x _ _ _)) :=  *)
+(*     M return nat -> nat -> (nat -> m M unit) -> m M unit in x. *)
+(* Arguments Foreach {M} : simpl never. *)
+(* Notation loopMonad := t. *)
+(* Coercion baseType : loopMonad >-> monad. *)
+(* Canonical baseType. *)
+(* End Exports. *)
+(* End MonadLoop. *)
+(* Export MonadLoop.Exports. *)
+
+Module MonadStateLoop.
+  Record mixin_of S (M : stateMonad S) : Type := Mixin {
+   foreach : nat -> nat -> (nat -> M unit) -> M unit ;
+  _ : forall m n body, foreach m (m + n.+1) body = Ret tt ;
+  _ : forall m body, foreach m m body = (body m);
+  _ : forall m n body, foreach (m.+1 + n) m body =
+     (body (m.+1 + n)) >> foreach (m + n) m body :> M unit
+}.
+Record class_of S (m : Type -> Type) := Class {
+  (* base : MonadLoop.class_of m ; *)
+  base : MonadState.class_of S m ;
+  (* base2 : MonadLoop.mixin_of (Monad.Pack (MonadState.base base)) ; *)
+  mixin : mixin_of (MonadState.Pack base)}.
+Structure t S : Type := Pack { m : Type -> Type ; class : class_of S m }.
+Definition baseType S (M : t S) : stateMonad S := MonadState.Pack (base (class M)).
+Module Exports.
+Notation loopStateMonad := t.
+(* Definition Break S (M : t S) : m M unit := *)
+(*   let: Pack _ (Class _ _ (Mixin x _ _ _ _)) := M return m M unit in x. *)
+(* Arguments Break {S M} : simpl never. *)
+Definition Foreach (M : t) : nat -> nat -> (nat -> m M unit) -> m M unit :=
+  let: Pack _ (Class _ (Mixin x _ _ _)) :=
+    M return nat -> nat -> (nat -> m M unit) -> m M unit in x.
+Coercion baseType : loopStateMonad >-> stateMonad.
+Canonical baseType.
+(* Definition l_of_loopstate S (M : loopStateMonad S) : loopMonad := *)
+(*   MonadLoop.Pack  (MonadLoop.Class (base2 (class M))). *)
+(* Canonical loop_of_loopstate. *)
+End Exports.
+End MonadStateLoop.
+Export MonadStateLoop.Exports.
+
+Section stateloop_lemmas.
+Variables (S : Type) (M : loopStateMonad S).
+Lemma loop0 m n (body : nat -> M unit) :
+  Foreach m (m + n.+1) body = Ret tt :> M _.
+Proof. by case: M body => ? [? []]. Qed.
+Lemma loop1 m (body : nat -> M unit) : Foreach m m body = body m.
+Proof. by case: M body => ? [? []]. Qed.
+Lemma loop2 m n body :
+  Foreach (m.+1 + n) m body =
+  (body (m.+1 + n) : M _) >> Foreach (m + n) m body :> M unit.
+Proof. by case: M body => ? [? []]. Qed.
+End stateloop_lemmas.
+
+Section examples.
+Variable (M : loopStateMonad nat).
+Set Printing All.
+Let example min max : M unit := Foreach max min (fun i : nat => (Get >> Ret tt : M _)).
+Print example.
+Let sum n : M unit := Foreach n O
+  (fun i : nat => (Get >>= (fun z => Put (z + i)) : M _)).
+
+Lemma sum_test n :
+  sum n = Get >>= (fun m => Put (m + sumn (iota 0 n.+1))).
+Proof.
+elim: n => [|n ih]; first by rewrite /sum loop1.
+rewrite {1}/sum -add1n loop2 bindA; bind_ext => m.
+rewrite -/(sum n) {}ih -bindA putget bindA bindretf putput.
+rewrite add1n -(addn1 n.+1) [in RHS]iota_add sumn_cat /=.
+by rewrite !(add0n,addn0) addnAC addnA.
+Qed.
+
+(* Let sumbreak n : M unit := Foreach n O *)
+(*  (fun i : nat => if i < 5 then Break else Get >>= (fun z => Put (z + i))). *)
+
+(* Let sumbreaknested n : M unit := Foreach n O *)
+(*   (fun i : nat => if i < 5 then Break else sum i). *)
+
+(* Let sumbreaknested2 n : M unit := Foreach n O *)
+(*   (fun i : nat => if i < 5 then Break else Foreach i 0 (fun y : nat => Get >>= (fun z => Put (z + i + y)))). *)
+
+End examples.
 
 Module MonadRun.
 Record mixin_of S (M : monad) : Type := Mixin {
